more progress

Lurk/New/Tag.lean
@@ -27,29 +27,30 @@ inductive ContTag
 open Lurk (F)
 
 def ExprTag.toF : ExprTag → F
-  | .num  => .ofNat 2
-  | .u64  => .ofNat 3
-  | .char => .ofNat 5
-  | .str  => .ofNat 7
-  | .comm => .ofNat 11
-  | .fun  => .ofNat 13
-  | .sym  => .ofNat 17
-  | .cons => .ofNat 19
+  | .num  => .ofNat 0
+  | .u64  => .ofNat 1
+  | .char => .ofNat 2
+  | .str  => .ofNat 3
+  | .comm => .ofNat 4
+  | .fun  => .ofNat 5
+  | .sym  => .ofNat 6
+  | .cons => .ofNat 7
 
 def ContTag.toF : ContTag → F
-  | .done => .ofNat 23
-  | .unOp .car => .ofNat 29
-  | .binOp₁ .add => .ofNat 31
-  | .binOp₁ .numEq => .ofNat 37
-  | .binOp₂ .add => .ofNat 41
-  | .binOp₂ .numEq => .ofNat 43
-  | .appFn => .ofNat 47
-  | .appArg => .ofNat 53
-  | .if => .ofNat 59
-  | .let => .ofNat 61
-  | .letrec => .ofNat 67
+  | .done => .ofNat 4096
+  | .unOp .car => .ofNat 4097
+  | .binOp₁ .add => .ofNat 4098
+  | .binOp₁ .numEq => .ofNat 4099
+  | .binOp₂ .add => .ofNat 4100
+  | .binOp₂ .numEq => .ofNat 4101
+  | .appFn => .ofNat 4102
+  | .appArg => .ofNat 4103
+  | .if => .ofNat 4104
+  | .let => .ofNat 4105
+  | .letrec => .ofNat 4106
 
-theorem ExprTag.toF_inj {t₁ t₂ : ExprTag} (h : t₁ ≠ t₂) : t₁.toF ≠ t₂.toF := sorry
+theorem ExprTag.toF_inj {t₁ t₂ : ExprTag} (h : t₁ ≠ t₂) : t₁.toF ≠ t₂.toF := by
+  cases t₁ <;> cases t₂ <;> simp only [h] <;> contradiction
 
 theorem ContTag.toF_inj {t₁ t₂ : ContTag} (h : t₁ ≠ t₂) : t₁.toF ≠ t₂.toF := sorry
 
