Lurk/New/LDON.lean
@@ -1,0 +1,10 @@
+import Lurk.Field
+
+inductive LDON
+  | num : Lurk.F → LDON
+  | u64 : UInt64 → LDON
+  | char : Char → LDON
+  | str : String → LDON
+  | sym : String → LDON
+  | cons : LDON → LDON → LDON
+  deriving Ord, BEq, Repr, Inhabited
