Lurk/New/Store.lean
@@ -1,25 +1,28 @@
 import Std.Data.RBMap
+import Poseidon.ForLurk
 import Lurk.New.Tag
+import Lurk.New.LDON
 
 open Lurk (F)
 
+section YoloPlaceholders
+
 def hash2 : F → F → F :=
-  fun a b => a * b * b
+  fun a b => .ofNat $ (Poseidon.Lurk.hash3 a 8192 b).norm
 
 def hash3 : F → F → F → F :=
-  fun a b c => a * b * b * c * c * c
+  fun a b c => .ofNat $ (Poseidon.Lurk.hash3 a b c).norm
 
 def hash4 : F → F → F → F → F :=
-  fun a b c d => a * b * b * c * c * c * d * d * d * d
+  fun a b c d => .ofNat $ (Poseidon.Lurk.hash4 a b c d).norm
  
 def hash6 : F → F → F → F → F → F → F :=
-  fun a b c d e f => a * b * b * c * c * c * d * d * d * d * e * e * e * e * e
-    * f * f * f * f * f * f
+  fun a b c d e f => hash2 (hash3 a b c) (hash3 d e f)
 
 def hash8 : F → F → F → F → F → F → F → F → F :=
-  fun a b c d e f g h => a * b * b * c * c * c * d * d * d * d * e * e * e * e * e
-    * f * f * f * f * f * f * g * g * g * g * g * g * g
-    * h * h * h * h * h * h * h * h
+  fun a b c d e f g h => hash2 (hash4 a b c d) (hash4 e f g h)
+
+end YoloPlaceholders
 
 structure ExprPtr where
   tag : ExprTag
@@ -33,8 +36,6 @@ structure ContPtr where
 
 inductive ExprPtrImg
   | cons : ExprPtr → ExprPtr → ExprPtrImg
-  | strCons : ExprPtr → ExprPtr → ExprPtrImg
-  | symCons : ExprPtr → ExprPtr → ExprPtrImg
   | «fun» : ExprPtr → ExprPtr → ExprPtr → ExprPtrImg
   | comm : F → ExprPtr → ExprPtrImg
 
@@ -72,19 +73,104 @@ end Symbol
 
 structure Store where
   exprData : RBMap ExprPtr ExprPtrImg compare
-  strs : RBMap ExprPtr String compare
-  syms : RBMap ExprPtr Symbol compare
-  strsMemo : RBMap String ExprPtr compare
-  symsMemo : RBMap Symbol ExprPtr compare
+
+  charsCache : RBMap (List Char) ExprPtr compare
+  stringsCashe : RBMap (List String) ExprPtr compare
+
+  ptrToStr : RBMap ExprPtr String compare
+  strToPtr : RBMap String ExprPtr compare
+
+  ptrToSym : RBMap ExprPtr Symbol compare
+  symToPtr : RBMap Symbol ExprPtr compare
 
   contData : RBMap ContPtr ContPtrImg compare
+  deriving Inhabited
 
 namespace Store
 
-def getStr (store : Store) : ExprPtr → Except String String := sorry
-def getSym (store : Store) : ExprPtr → Except String Symbol := sorry
+abbrev StoreM := EStateM String Store
 
-def putStr (store : Store) : String → (ExprPtr × Store) := sorry
-def putSym (store : Store) : Symbol → (ExprPtr × Store) := sorry
+@[inline] def addToExprStore (ptr : ExprPtr) (img : ExprPtrImg) : StoreM ExprPtr :=
+  modifyGet fun c => (ptr, { c with exprData := c.exprData.insert ptr img })
+
+@[inline] def addToContStore (ptr : ContPtr) (img : ContPtrImg) : StoreM ContPtr :=
+  modifyGet fun c => (ptr, { c with contData := c.contData.insert ptr img })
+
+def putChars (cs : List Char) : StoreM ExprPtr := do
+  match (← get).charsCache.find? cs with
+  | some ptr => pure ptr
+  | none =>
+    let ptr ← match cs with
+      | [] => pure ⟨.str, F.zero⟩
+      | c :: cs =>
+        let headPtr := ⟨.char, .ofNat c.toNat⟩
+        let tailPtr ← putChars cs
+        addToExprStore
+          ⟨.str, hash4 headPtr.tag.toF headPtr.val tailPtr.tag.toF tailPtr.val⟩
+          (.cons headPtr tailPtr)
+    modifyGet fun stt =>
+      (ptr, { stt with charsCache := stt.charsCache.insert cs ptr })
+
+def putStrings (ss : List String) : StoreM ExprPtr := do
+  match (← get).stringsCashe.find? ss with
+  | some ptr => return ptr
+  | none =>
+    let ptr ← ss.foldrM (init := ⟨.sym, F.zero⟩) fun s acc => do
+      let strPtr ← putChars s.data
+      addToExprStore
+        ⟨.sym, hash4 strPtr.tag.toF strPtr.val acc.tag.toF acc.val⟩
+        (.cons strPtr acc)
+    modifyGet fun stt =>
+      (ptr, { stt with stringsCashe := stt.stringsCashe.insert ss ptr })
+
+def putStr (str : String) : StoreM ExprPtr := do
+  match (← get).strToPtr.find? str with
+  | some ptr => return ptr
+  | none =>
+    let ptr ← putChars str.data
+    modifyGet fun store => (ptr, { store with
+      ptrToStr := store.ptrToStr.insert ptr str
+      strToPtr := store.strToPtr.insert str ptr })
+
+def putSym (sym : Symbol) : StoreM ExprPtr := do
+  match (← get).symToPtr.find? sym with
+  | some ptr => return ptr
+  | none =>
+    let ptr ← putStrings sym.telescope
+    modifyGet fun store => (ptr, { store with
+      ptrToSym := store.ptrToSym.insert ptr sym
+      symToPtr := store.symToPtr.insert sym ptr })
+
+def hashLDON : LDON → StoreM ExprPtr
+  | .num n => pure ⟨.num, n⟩
+  | .u64 n => pure ⟨.u64, .ofNat n.val⟩
+  | .char n => pure ⟨.char, .ofNat n.toNat⟩
+  | .str s => putChars s.data
+  | .sym s => putStrings [s, "LURK"]
+  | .cons car cdr => do
+    let car ← hashLDON car
+    let cdr ← hashLDON cdr
+    addToExprStore
+      ⟨.cons, hash4 car.tag.toF car.val cdr.tag.toF cdr.val⟩
+      (.cons car cdr)
+
+def hideLDON (secret : F) (x : LDON) : StoreM F := do
+  let ptr ← hashLDON x
+  let hash := hash3 secret ptr.tag.toF ptr.val
+  discard $ addToExprStore ⟨.comm, hash⟩ (.comm secret ptr)
+  return hash
+
+def getStr (ptr : ExprPtr) : StoreM String := do
+  match (← get).ptrToStr.find? ptr with
+  | some str => return str
+  | none => sorry -- pull from store and then memoize
+
+def getSym (ptr : ExprPtr) : StoreM Symbol := do
+  match (← get).ptrToSym.find? ptr with
+  | some sym => return sym
+  | none => sorry -- pull from store and then memoize
 
 end Store
+
+def ExprPtr.isNil (ptr : ExprPtr) : Store.StoreM Bool :=
+  return ptr == (← Store.putSym .nil)
